Prove distributed adequacy theorem for goose lang
Also introduces a notion of equivalence on irisG and perennialG type
class instances and shows that wpc and wpr respect that notion of
equivalence. Slight tweaks made to wpr in order to show this is true.

src/goose_lang/lifting.v
@@ -258,20 +258,20 @@ Record heap_local_names := {
   heap_local_trace_names : tr_names;
 }.
 
-Definition heap_update_names Σ (hG : heapG Σ) (names: heap_names) :=
+Definition heap_update_local_names Σ (hG : heapG Σ) (names: heap_local_names) :=
   {| heapG_invG := heapG_invG;
      heapG_crashG := heapG_crashG;
-     heapG_ffiG := ffi_update_local Σ (heapG_ffiG) (heap_ffi_local_names names);
-     heapG_na_heapG := na_heapG_update (heapG_na_heapG) (heap_heap_names names);
-     heapG_traceG := traceG_update Σ (heapG_traceG) (heap_trace_names names)
+     heapG_ffiG := ffi_update_local Σ (heapG_ffiG) (heap_local_ffi_local_names names);
+     heapG_na_heapG := na_heapG_update (heapG_na_heapG) (heap_local_heap_names names);
+     heapG_traceG := traceG_update Σ (heapG_traceG) (heap_local_trace_names names)
  |}.
 
-Definition heap_update Σ (hG : heapG Σ) (Hinv: invG Σ) (Hcrash : crashG Σ) (names: heap_names) :=
+Definition heap_update_local Σ (hG : heapG Σ) (Hinv: invG Σ) (Hcrash : crashG Σ) (names: heap_local_names) :=
   {| heapG_invG := Hinv;
      heapG_crashG := Hcrash;
-     heapG_ffiG := ffi_update_local Σ (heapG_ffiG) (heap_ffi_local_names names);
-     heapG_na_heapG := na_heapG_update (heapG_na_heapG) (heap_heap_names names);
-     heapG_traceG := traceG_update Σ (heapG_traceG) (heap_trace_names names)
+     heapG_ffiG := ffi_update_local Σ (heapG_ffiG) (heap_local_ffi_local_names names);
+     heapG_na_heapG := na_heapG_update (heapG_na_heapG) (heap_local_heap_names names);
+     heapG_traceG := traceG_update Σ (heapG_traceG) (heap_local_trace_names names)
  |}.
 
 Definition heap_get_names Σ (hG : heapG Σ) : heap_names :=
@@ -281,10 +281,22 @@ Definition heap_get_names Σ (hG : heapG Σ) : heap_names :=
      heap_trace_names := trace_tr_names;
  |}.
 
+Definition heap_get_local_names Σ (hG : heapG Σ) : heap_local_names :=
+  {| heap_local_heap_names := na_heapG_get_names (heapG_na_heapG);
+     heap_local_ffi_local_names := ffi_get_local_names Σ (heapG_ffiG);
+     heap_local_trace_names := trace_tr_names;
+ |}.
+
+Definition heap_extend_local_names (names : heap_local_names) (namesg: ffi_global_names) : heap_names :=
+  {| heap_heap_names := heap_local_heap_names names;
+     heap_ffi_local_names := heap_local_ffi_local_names names;
+     heap_trace_names := heap_local_trace_names names;
+     heap_ffi_global_names := namesg |}.
+
 Lemma heap_get_update Σ hG :
-  heap_update_names Σ hG (heap_get_names _ hG) = hG.
+  heap_update_local_names Σ hG (heap_get_local_names _ hG) = hG.
 Proof.
-  rewrite /heap_update_names/heap_get_names/na_heapG_update/na_heapG_get_names ffi_get_update //=.
+  rewrite /heap_update_local_names/heap_get_local_names/na_heapG_update/na_heapG_get_names ffi_get_update //=.
   destruct hG as [??? [] []]; eauto.
 Qed.
 
@@ -310,14 +322,14 @@ Global Program Instance heapG_irisG `{!heapG Σ}:
 Next Obligation. intros. eauto. Qed.
 
 Lemma heap_get_update' Σ hG :
-  heap_update Σ hG (iris_invG) (iris_crashG) (heap_get_names _ hG) = hG.
+  heap_update_local Σ hG (iris_invG) (iris_crashG) (heap_get_local_names _ hG) = hG.
 Proof.
-  rewrite /heap_update/heap_get_names/na_heapG_update/na_heapG_get_names ffi_get_update //=.
+  rewrite /heap_update_local/heap_get_local_names/na_heapG_update/na_heapG_get_names ffi_get_update //=.
   destruct hG as [??? [] []]; eauto.
 Qed.
 
 Lemma heap_update_invG Σ hG Hinv Hc names:
-  @iris_invG _ _ (@heapG_irisG _ (heap_update Σ hG Hinv Hc names)) = Hinv.
+  @iris_invG _ _ (@heapG_irisG _ (heap_update_local Σ hG Hinv Hc names)) = Hinv.
 Proof. rewrite //=. Qed.
 
 (** The tactic [inv_head_step] performs inversion on hypotheses of the shape
