src/goose_lang/wpr_lifting.v
@@ -13,12 +13,13 @@ Context `{ffi_semantics: ext_semantics}.
 Context {ext_tys: ext_types ext}.
 Context `{!ffi_interp ffi}.
 
-Canonical Structure heap_namesO := leibnizO heap_names.
+Canonical Structure heap_local_namesO := leibnizO heap_local_names.
 
-Program Global Instance heapG_perennialG `{!heapG Σ} : perennialG goose_lang goose_crash_lang heap_namesO Σ :=
+Program Global Instance heapG_perennialG `{!heapG Σ} :
+  perennialG goose_lang goose_crash_lang heap_local_namesO Σ :=
 {
   perennial_irisG := λ Hcrash hnames,
-                     @heapG_irisG _ _ _ _ _ (heap_update _ _ _ Hcrash (@pbundleT _ _ hnames));
+                     @heapG_irisG _ _ _ _ _ (heap_update_local _ _ _ Hcrash (@pbundleT _ _ hnames));
   perennial_crashG := λ _ _, eq_refl;
   perennial_num_laters_per_step := λ n, n
 }.
@@ -27,10 +28,10 @@ Next Obligation. eauto. Qed.
 
 Definition wpr `{hG: !heapG Σ} `{hC: !crashG Σ} (s: stuckness) (k: nat) (E: coPset)
   (e: expr) (recv: expr) (Φ: val → iProp Σ) (Φinv: heapG Σ → iProp Σ) (Φr: heapG Σ → val → iProp Σ) :=
-  wpr s k hC ({| pbundleT := heap_get_names Σ _ |}) E e recv
+  wpr s k hC ({| pbundleT := heap_get_local_names Σ _ |}) E e recv
               Φ
-              (λ Hc names, Φinv (heap_update _ _ _ Hc (@pbundleT _ _ names)))
-              (λ Hc names v, Φr (heap_update _ _ _ Hc (@pbundleT _ _ names)) v).
+              (λ Hc names, Φinv (heap_update_local _ _ _ Hc (@pbundleT _ _ names)))
+              (λ Hc names v, Φr (heap_update_local _ _ _ Hc (@pbundleT _ _ names)) v).
 
 
 Section wpr.
@@ -70,11 +71,11 @@ Lemma idempotence_wpr `{!ffi_interp_adequacy} s k E1 e rec Φx Φinv Φrx Φcx:
 Proof.
   iIntros "Hwpc #Hidemp".
   iApply (idempotence_wpr s k E1 e rec _ _ _
-                          (λ Hc names, Φcx (heap_update _ _ _ Hc (@pbundleT _ _ names)))
+                          (λ Hc names, Φcx (heap_update_local _ _ _ Hc (@pbundleT _ _ names)))
                                                     with "[Hwpc] [Hidemp]"); first auto.
   { rewrite //= heap_get_update' //=. }
   { iModIntro. iIntros (?? σ_pre_crash g σ_post_crash Hcrash ns κs ?) "H".
-    iSpecialize ("Hidemp" $! (heap_update _ _ _ _ _) with "[//] [//] H").
+    iSpecialize ("Hidemp" $! (heap_update_local _ _ _ _ _) with "[//] [//] H").
     {
       rewrite /state_interp.
       iIntros "(_&Hffi_old&Htrace_auth&Horacle_auth) Hg".
@@ -82,13 +83,12 @@ Proof.
       iMod (ffi_crash _ σ_pre_crash.(world) σ_post_crash.(world) with "Hffi_old Hg") as (ffi_names) "(Hw&Hg&Hcrel&Hc)".
       { inversion Hcrash; subst; eauto. }
       iMod (trace_reinit _ σ_post_crash.(trace) σ_post_crash.(oracle)) as (name_trace) "(Htr&Htrfrag&Hor&Hofrag)".
-      set (hnames := {| heap_heap_names := name_na_heap;
-                        heap_ffi_local_names := ffi_names;
-                        heap_ffi_global_names := ffi_get_global_names _  (heapG_ffiG);
-                        heap_trace_names := name_trace |}).
+      set (hnames := {| heap_local_heap_names := name_na_heap;
+                        heap_local_ffi_local_names := ffi_names;
+                        heap_local_trace_names := name_trace |}).
       iModIntro.
       iNext. iIntros (Hc' ?) "HNC".
-      set (hG' := (heap_update _ _ _ Hc' hnames)).
+      set (hG' := (heap_update_local _ _ _ Hc' hnames)).
       iSpecialize ("Hidemp" $! σ_pre_crash.(world) σ_post_crash.(world) hG' with "[Hcrel] [Hc]").
       { rewrite //= ffi_update_update //=. }
       { rewrite //= ffi_update_update //=. }
