src/goose_lang/recovery_adequacy.v
@@ -18,22 +18,30 @@ Theorem heap_recv_adequacy `{ffi_sem: ext_semantics} `{!ffi_interp ffi} {Hffi_ad
   recv_adequate (CS := goose_crash_lang) s e r σ g (λ v _ _, φ v) (λ v _ _, φr v) (λ σ _, φinv σ).
 Proof.
   intros Hwp.
-  eapply (wp_recv_adequacy_inv _ _ _ heap_namesO _ _ _ _ _ _ _ _ _ (λ names0 Hinv Hc names, Φinv (heap_update _ (heap_update_pre _ _ Hinv Hc (@pbundleT _ _ names0)) Hinv Hc (@pbundleT _ _ names))) (λ n, n)).
+  eapply (wp_recv_adequacy_inv _ _ _ heap_local_namesO _ _ _ _ _ _ _ _ _
+           (* (λ names0 Hinv Hc names, ∃ namesg, Φinv (heap_update_local _
+                                         (heap_update_pre _ _ Hinv Hc (heap_extend_local_names (@pbundleT _ _ names) namesg)) Hinv Hc (@pbundleT _ _ names)))%I *) (λ n, n)).
   iIntros (???) "".
   iMod (na_heap_name_init tls σ.(heap)) as (name_na_heap) "Hh".
   iMod (ffi_name_global_init _ _ g) as (ffi_namesg) "(Hgw&_)"; first auto.
   iMod (ffi_name_init _ _ σ.(world) g with "Hgw") as (ffi_names) "(Hw&Hgw&Hstart)"; first auto.
   iMod (trace_name_init σ.(trace) σ.(oracle)) as (name_trace) "(Htr&Htrfrag&Hor&Hofrag)".
+  (*
+  set (hnames := {| heap_heap_names := name_na_heap;
+                      heap_ffi_local_names := ffi_names;
+                      heap_ffi_global_names := ffi_namesg;
+                      heap_trace_names := name_trace |}).
+   *)
   set (hnames := {| heap_heap_names := name_na_heap;
                       heap_ffi_local_names := ffi_names;
                       heap_ffi_global_names := ffi_namesg;
                       heap_trace_names := name_trace |}).
   set (hG := heap_update_pre _ hPre Hinv Hc hnames).
-  iExists ({| pbundleT := hnames |}).
+  iExists ({| pbundleT := heap_get_local_names Σ hG |}).
   iExists
-    (λ t σ nt, let _ := heap_update Σ hG Hinv Hc (@pbundleT _ _ t) in
+    (λ t σ nt, let _ := heap_update_local Σ hG Hinv Hc (@pbundleT _ _ t) in
                state_interp σ nt)%I,
-    (λ t g ns κs, let _ := heap_update Σ hG Hinv Hc (@pbundleT _ _ t) in
+    (λ t g ns κs, let _ := heap_update_local Σ hG Hinv Hc (@pbundleT _ _ t) in
                   global_state_interp g ns κs).
   iExists _. (* (λ Hc t, λ (σ0 : state) (_ : nat) (κs0 : list observation) (_ : nat),
                                               lifting.heapG_irisG_obligation_1 Σ
@@ -43,14 +51,16 @@ Proof.
   iExists _.
   iExists _.
   iExists _.
+  iExists ((λ names0 Hinv Hc names, Φinv (heap_update_local _ hG Hinv Hc (@pbundleT _ _ names)))).
   iMod (Hwp hG with "[$] [$] [$]") as "(#H1&#H2&Hwp)".
   iModIntro.
   iSplitR.
   { iModIntro. iIntros (??) "Hσ".
     iApply ("H1" with "[Hσ]").
     iExactEq "Hσ". do 2 f_equal.
-    rewrite /heap_update/hG/heap_update_pre//=. f_equal.
-    rewrite ffi_update_pre_update. eauto.
+    rewrite /heap_update_local/hG/heap_update_pre//=. f_equal.
+    rewrite ?ffi_update_pre_update.
+    rewrite ffi_update_pre_get_local //=.
   }
   iSplitR.
   {
@@ -59,13 +69,13 @@ Proof.
     { iExactEq "H".
       f_equal.
     }
-    iModIntro. iIntros (??) "H". iSpecialize ("H3" with "H"); eauto.
+    iModIntro. iIntros (??) "H". iSpecialize ("H3" with "[H]"); eauto.
   }
   iFrame. rewrite /hG//=.
   rewrite ffi_update_pre_update //=. iFrame.
   rewrite /wpr. rewrite /hG//=.
-  rewrite heap_update_pre_get.
-  rewrite //=.
+  iFrame.
+  rewrite ffi_update_pre_get_local //=. iFrame.
   Unshelve.
   - eauto.
   - exact O.
