src/program_logic/recovery_adequacy.v
@@ -216,7 +216,7 @@ Proof.
   iModIntro.
   destruct s0.
   - iIntros (Hc') "HNC". iSpecialize ("H" $! Hc' with "[$]").
-    iMod "H" as (t' Heq' Heqpf') "(Hσ&Hg&Hr&HNC)".
+    iMod "H" as (t' Heqpf') "(Heq&Hσ&Hg&Hr&HNC)".
     iDestruct "Hr" as "(_&Hr)".
     simpl in *.
     iPoseProof (IH with "[Hσ] [Hg] Hr [] [] HNC") as "H"; eauto.
@@ -229,7 +229,7 @@ Proof.
     assert ((S (n' + ncurr + sum_crash_steps ns')) =
         (ncurr + S (n' + sum_crash_steps ns'))) as -> by lia. auto.
   - iIntros (Hc') "HNC".
-    iMod ("H" $! Hc' with "[$]") as (t' Heq' Heqpf') "(Hσ&Hg&Hr&HNC)".
+    iMod ("H" $! Hc' with "[$]") as (t' Heqpf') "(Heq&Hσ&Hg&Hr&HNC)".
     iExists t'.
     iAssert (□Φinv' Hc' t')%I as "#Hinv'".
     { iDestruct "Hr" as "(Hr&_)".
@@ -411,12 +411,13 @@ Proof.
   - constructor; naive_solver.
 Qed.
 
-Corollary wp_recv_adequacy_inv Σ Λ CS (T: ofe) `{!invPreG Σ} `{!crashPreG Σ} s k e r σ g φ φr φinv Φinv f:
+Corollary wp_recv_adequacy_inv Σ Λ CS (T: ofe) `{!invPreG Σ} `{!crashPreG Σ} s k e r σ g φ φr φinv f:
   (∀ `{Hinv : !invG Σ} `{Hc: !crashG Σ} κs,
      ⊢ |={⊤}=> ∃ (t: pbundleG T Σ)
          (stateI : pbundleG T Σ → state Λ → nat → iProp Σ)
          (global_stateI : pbundleG T Σ → global_state Λ → nat → list (observation Λ) → iProp Σ)
-         (fork_post : pbundleG T Σ → val Λ → iProp Σ) Hpf1 Hpf1' Hpf2 Hpf3,
+         (fork_post : pbundleG T Σ → val Λ → iProp Σ) Hpf1 Hpf1' Hpf2 Hpf3
+         Φinv,
         let _ : perennialG Λ CS _ Σ :=
             PerennialG _ _ T Σ
               (λ Hc t,
@@ -436,7 +437,8 @@ Proof.
               (crash_adequacy.steps_sum f (sum_crash_steps ns') n')
               (S $ S $ (f (n' + sum_crash_steps ns' + 0))))=> Hinv Hc.
   iIntros "HNC".
-  iMod (Hwp Hinv Hc κs) as (t stateI global_stateI Hfork_post Hpf1 Hpf1' Hpf2 Hpf3) "(#Hinv1&#Hinv2&Hσ&Hg&H)".
+  iMod (Hwp Hinv Hc κs) as (t stateI global_stateI Hfork_post Hpf1 Hpf1' Hpf2 Hpf3) "H".
+  iDestruct "H" as (Φinv) "(#Hinv1&#Hinv2&Hσ&Hg&H)".
   iModIntro.
   set (pG :=
           PerennialG _ _ T Σ
